Proofs/fact.v
@@ -6,7 +6,7 @@ Import proofmode notation.
 
 Definition factI : heap_lang.expr :=
   rec: "factI" "n" :=
-    if: "n" < #1 then #1 else "factI" * ("n" - #1)
+    if: "n" < #1 then #1 else "n" * "factI" ("n" - #1)
     .
 
 End iris.
@@ -19,61 +19,112 @@ Require Import Vloc.CCode.fact.
 #[local] Instance CompSpecs : compspecs. make_compspecs prog. Defined.
 Definition Vprog : varspecs.  mk_varspecs prog. Defined.
 
-(* here, the refines we had before won't work... *)
-Definition int_relate vVST vHL :=
-  (!! (exists n : Z, vVST = Vint (Int.repr n) /\ vHL = LitV (heap_lang.LitInt n%Z)) && emp)%logic.
 
+Definition nat_relate n vVST vHL :=
+  (((Int.min_signed <= n <= Int.max_signed)%Z -> (vVST = Vint (Int.repr n))%Z) /\ vHL = LitV (heap_lang.LitInt n%Z)).
+
+(* for simplicity, we're ignoring out of bounds errors here *)
+Fixpoint fact n : nat :=
+  match n with
+  | O => 1
+  | S (n') => n * (fact n')
+  end.
+
+(* here, the refines we had before won't work... *)
 Definition fspec :=
   DECLARE _factorial
   WITH gv: globals, ctx: ref_id, n : Z
   PRE [ tint ]
-    PROP((n <= Int.max_signed)%Z)
+    PROP((Int.min_signed <= n <= Int.max_signed)%Z)
     PARAMS(Vint (Int.repr n))
     GLOBALS()
     SEP(refines_right ctx (App iris.factI (Val (LitV (LitInt n)))))
   POST [ tint ] 
-    EX v' : ival, EX v : val,
-    PROP()
+    EX n : Z, EX v' : ival, EX v : val,
+    PROP(nat_relate n v v')
     RETURN(v)
-    SEP(refines_right ctx (ectxi_language.of_val v') * int_relate v v').
+    SEP((refines_right ctx (ectxi_language.of_val v'))).
 
 Definition Gprog : funspecs := [fspec].
 
-Lemma one_plus_zero : semax_body Vprog Gprog f_factorial fspec.
+
+Lemma fact_lemma : semax_body Vprog Gprog f_factorial fspec.
 Proof.
   start_function. 
-  step_pure_r ctx.
-  forward.
-  destruct (eq_dec n 0).
-  - forward_for_simple_bound n (EX i:Z,
-      PROP()
-      LOCAL(temp _acc (Vint (Int.repr 1)); temp _n (Vint (Int.repr n)))
-      SEP(refines_right ctx (App
+  forward_if (
+    PROP((n >= 1)%Z) 
+    LOCAL(temp _n (Vint (Int.repr n))) 
+    SEP(refines_right ctx
+       (BinOp MultOp (Val (LitV (LitInt n)))
+          (App
              (Val
                 (RecV "factI" "n"
                    (If (BinOp LtOp (Var "n") (Val (LitV (LitInt 1))))
                       (Val (LitV (LitInt 1)))
-                      (BinOp MultOp (Var "factI")
-                         (BinOp MinusOp (Var "n") (Val (LitV (LitInt 1))))))))
-             (Val (LitV (LitInt n)))))
-    ).
-    entailer!.
-    lia.
-    step_pure_r ctx.
-    step_pure_r ctx.
-    step_pure_r ctx.
-    step_pure_r ctx.
+                      (BinOp MultOp (Var "n")
+                         (App (Var "factI")
+                            (BinOp MinusOp (Var "n") (Val (LitV (LitInt 1)))))))))
+             (Val (LitV (LitInt (n - 1)))))))
+  ).
+  (* n is zero or less *)
+  {
+    (* step hl to right form *)
+    do 5 step_pure_r ctx.
     forward.
+    simpl.
+    replace (Z.pos (1 * 1)) with (Z.pos 1) by lia.
+    Exists 1%Z.
     Exists (LitV (heap_lang.LitInt 1%Z)).
     Exists (Vint (Int.repr 1)).
-    iIntros "H".
-    iSplit; first iPureIntro; auto.
-    iSplit; last iPureIntro; eauto.
-
-  - forward_for_simple_bound n (EX i:Z, 
-      PROP()
-      LOCAL(temp _acc (Vint (Int.repr 1)); temp _n (Vint (Int.repr n)))
-      SEP()
-    )%assert.
-
+    entailer!.
+    unfold nat_relate.
+    auto.
+  }
+  {
+    (* step hl through 1 cycle *)
+    do 6 step_pure_r ctx.
+    forward.
+    entailer!.
+  }
+  Intros.
+  forward_call (gv, add_to_ctx ctx [BinOpRCtx MultOp (Val (LitV (LitInt n)))], (n-1)%Z); try lia.
+  {
+    unfold iris.factI.
+    (* we need to step the rhs once to handle the fact that it didn't recure fully? *)
+    replace (App (heap_lang.Rec _ _ _)) with 
+      (App (Val
+           (RecV "factI" "n"
+              (If (BinOp LtOp (Var "n") (Val (LitV (LitInt 1))))
+                 (Val (LitV (LitInt 1)))
+                 (BinOp MultOp (Var "n")
+                    (App (Var "factI")
+                       (BinOp MinusOp (Var "n") (Val (LitV (LitInt 1)))))))))).
+     2:{
+       (* TODO: figure out how to turn heap_lang.Rec into Val (RecV ... or rewrite the program *)
+       admit.
+     }
+    replace (BinOp _ _ _) with (fill [BinOpRCtx MultOp (Val (LitV (LitInt n)))] (App
+        (Val
+           (RecV "factI" "n"
+              (If (BinOp LtOp (Var "n") (Val (LitV (LitInt 1))))
+                 (Val (LitV (LitInt 1)))
+                 (BinOp MultOp (Var "n")
+                    (App (Var "factI")
+                       (BinOp MinusOp (Var "n") (Val (LitV (LitInt 1)))))))))
+        (Val (LitV (LitInt (n - 1)))))) by by rewrite ? fill_app.
+    rewrite refines_right_add_ctx.
+    cancel.
+  }
+  (* extract recursive value *)
+  Intros ret.
+  destruct ret as [[rn iret] vret]; simpl; simpl in H1. 
+  rewrite <- refines_right_add_ctx; simpl.
+  forward.
+  - unfold nat_relate in H1; destruct H1 as [Hl Hr].
+    subst.
+    entailer!.
+    (* TODO: how to get bounds? I can try to add it to the implication but then other things break *)
+    admit.
+  - unfold nat_relate in H1; destruct H1 as [Hl Hr].
+    Exists 
 Admitted.
